%https://tex.stackexchange.com/questions/37581/latex-figures-side-by-side
% put a double figure side by side

%\documentclass[12pt]{report}
%\documentclass[12pt]{extreport}
\documentclass[14pt]{extarticle}
%\documentclass{memoir}

\usepackage{graphicx}
\usepackage{setspace}
\usepackage{amsmath,amssymb}
\usepackage{IEEEtrantools}
\usepackage{cancel}
\usepackage[font=small,labelfont=bf]{caption}
\usepackage{subcaption}
\usepackage{enumitem}

\usepackage{verbatim}
%\usepackage{textcomp}
\usepackage{eurosym}


\usepackage[T1]{fontenc}
\usepackage[utf8]{inputenc}
\usepackage[italian]{babel}


%\usepackage{imakeidx}%
%\makeindex[program=xindy]%, options=-C utf8 -L portuguese]%
\usepackage{makeidx}
\makeindex




\usepackage{geometry}
 \geometry{
 a4paper,
 total={170mm,264mm},
 left=8mm,
 right=8mm,
 top=10mm,
 bottom=10mm
 }

\begin{document}

%\backmatter
%text\index{test}
%\printindex



\pagenumbering{gobble}

\begin{center}
{\bf Circumference equation from two points (po and po) and radius (ra)}
\end{center}

point0: $P(x0, y0)$\\
point1: $P(x1, y1)$\\

\begin{eqnarray}
	x_0^2 + y_0^2 + ax_0 + bx_0 + c = 0\qquad - \\
	x_1^2 + y_1^2 + ax_1 + bx_1 + c = 0\qquad =
\end{eqnarray}

\hrule

\begin{eqnarray}
	\left(x_0 + x_1 + a\right)\left(x_0 - x_1\right) + \left( y_0 + y_1 + b\right)\left(y_0 - y_1\right) = 0\\
\end{eqnarray}

\begin{eqnarray}
	b & = & - \frac{\left(x_0 + x_1 + a\right)\left(x_0 - x_1\right)}{y_0 - y_1} - \left(y_0 + y_1\right)\\
	b & = & -a\frac{x_0-x_1}{y_0 - y1} - \frac{x_0^2 -x_1^2 + y_0^2 - y_1^2}{y_0 - y_1}	
\end{eqnarray}

\begin{eqnarray}
	\gamma & = & - \frac{x_0 - x_1}{y_0 - y_1}\\
	\delta & = & -\frac{x_0^2 - x_1^2 + y_0^2 - y_1^2}{y_0 - y_1}
\end{eqnarray}


\begin{eqnarray}
	\Rightarrow\qquad b = \gamma a + \delta
\end{eqnarray}


\newpage



\begin{eqnarray}
	x_0^2 + y_0^2 + ax_0 + bx_0 + c = 0\qquad + \\
	x_1^2 + y_1^2 + ax_1 + bx_1 + c = 0\qquad =
\end{eqnarray}


\hrule

\begin{eqnarray}
	x_0^2 + x_1^2 + y_0^2 + y_1^2 + a(x_0 + x_1) + (\gamma a + \delta)(y_0 + y_1) - 2R^2 + \frac{a^2}{2} + \frac{b^2}{2} = 0\\
	\Rightarrow a_rx^2 + 2b_rx + c_r = 0
\end{eqnarray}

\begin{eqnarray}
	a_{1,2} = \frac{-b_r \pm \sqrt{b_r^2 - a_rc_r}}{a_r}
\end{eqnarray}


\end{document}